Data/Lib.hs
@@ -2,11 +2,6 @@ module Data.Lib where
 
 import qualified Prelude
 import qualified Data.List
-import qualified Data.Specif as Specif
-
-
-__ :: any
-__ = Prelude.error "Logical or arity value used"
 
 undefined :: a1
 undefined =
@@ -18,21 +13,18 @@ fromMaybe d mx =
    Prelude.Just x -> x;
    Prelude.Nothing -> d}
 
-existT_in_cons :: a1 -> ([] a1) -> (Specif.Coq_sigT a1 ()) -> Specif.Coq_sigT
-                  a1 ()
-existT_in_cons a l x =
+exist_in_cons :: a1 -> ([] a1) -> a1 -> a1
+exist_in_cons a l x =
   case l of {
    [] -> Prelude.error "absurd case";
-   (:) a0 l0 ->
-    case x of {
-     Specif.Coq_existT x0 _ -> Specif.Coq_existT x0 __}}
+   (:) a0 l0 -> x}
 
-list_membership :: ([] a1) -> [] (Specif.Coq_sigT a1 ())
+list_membership :: ([] a1) -> [] a1
 list_membership l =
   case l of {
    [] -> [];
-   (:) x xs -> (:) (Specif.Coq_existT x __)
-    ((Prelude.map) (existT_in_cons x xs) (list_membership xs))}
+   (:) x xs -> (:) x
+    ((Prelude.map) (exist_in_cons x xs) (list_membership xs))}
 
 safe_hd :: ([] a1) -> a1
 safe_hd xs =
